separate out expr for reuse

src/implang_cont.v
@@ -1,28 +1,12 @@
 From stdpp Require Export binders strings.
 From stdpp Require Import gmap.
 From iris.algebra Require Export ofe.
+From iris_simp_lang Require Export implang_expr.
 From iris.prelude Require Import options.
 Open Scope Z.
 From RecordUpdate Require Import RecordSet.
 Import RecordSetNotations.
 
-
-Inductive bin_op :=
-  | PlusOp
-  | EqOp.
-
-Inductive un_op :=
-  | DerefOp.
-
-Inductive expr :=
-  (* Values *)
-  | Num (n : Z)
-  (* local variable *)
-  | Var (x : string)
-  (* Pure operations *)
-  | BinOp (op : bin_op) (e1 e2 : expr)
-  | UnOp (op : un_op) (e : expr)
-.
 
 (* s ::= skip | x := e | x := alloc | *e := e | s;s | if (e){s}else{s}
          | while(e){s} | x := f(\vec{e}) | return e 
@@ -44,7 +28,6 @@ Inductive stmt :=
 Inductive func :=
   | Func (func_params : list string) (func_body : stmt).
 
-Bind Scope expr_scope with expr.
 Bind Scope stmt_scope with stmt.
 Bind Scope func_scope with func.
 
@@ -55,13 +38,6 @@ We will now do a bunch of boring work to prove that expressions have decidable
 equality and are countable for technical reasons.
 |*)
 
-Global Instance bin_op_eq_dec : EqDecision bin_op.
-Proof. solve_decision. Defined.
-Global Instance un_op_eq_dec : EqDecision un_op.
-Proof. solve_decision. Defined.
-Lemma expr_eq_dec (e1 e2: expr) : Decision (e1 = e2).
-Proof. solve_decision. Defined.
-Global Instance expr_eq_dec' : EqDecision expr := expr_eq_dec.
 Lemma stmt_eq_dec (s1 s2: stmt) : Decision (s1 = s2).
 Proof. solve_decision. Defined.
 Global Instance stmt_eq_dec' : EqDecision stmt := stmt_eq_dec.
@@ -69,32 +45,7 @@ Lemma func_eq_dec (f1 f2: func) : Decision (f1 = f2).
 Proof. solve_decision. Defined.
 Global Instance func_eq_dec' : EqDecision func := func_eq_dec.
 
-Definition Bool (b:bool) : expr := Num (if b then 1 else 0).
-
 (* semantics *)
-Definition loc := Z.
-
-Inductive val :=
-  | NumV (n : Z)
-  | LocV (l : loc).
-
-Lemma val_eq_dec (v1 v2 : val) : Decision (v1 = v2).
-Proof. solve_decision. Defined.
-Global Instance val_eq_dec' : EqDecision val := val_eq_dec.
-
-Definition BoolV (b:bool) : val := NumV (if b then 1 else 0).
-
-Definition bin_op_eval (op: bin_op) (v1 v2: val) : option val :=
-  match op with
-  | PlusOp => match v1, v2 with
-              | NumV n1, NumV n2 =>
-                Some (NumV (n1 + n2))
-              | LocV n1, NumV n2 | NumV n1, LocV n2 =>
-                Some (LocV (n1 + n2))
-              | _, _ => None
-              end
-  | EqOp => Some (BoolV $ bool_decide (v1 = v2))
-  end.
 
 (* make into a list? *)
 Inductive cont :=
@@ -130,8 +81,6 @@ Record state : Type := {
 (** the language interface needs these things to be inhabited, I believe *)
 Global Instance state_inhabited : Inhabited state :=
   populate {| ρ := inhabitant; m := inhabitant; k := Kstop  |}.
-Global Instance val_inhabited : Inhabited val := populate (NumV 0).
-Global Instance expr_inhabited : Inhabited expr := populate (Num 0).
 
 #[export] Instance settable_state : Settable state :=
   settable! Build_state <ρ; m; k>. 
@@ -139,41 +88,6 @@ Example state_upd_env (f: gmap string val → gmap string val) (s: state) : stat
   s <| ρ ::= f |>.
 Example state_upd_heap (f: gmap loc val → gmap loc val) (s: state) : state :=
   s <| m ::= f |>.
-
-
-Inductive eval_expr : expr → gmap string val → gmap loc val → val → Prop :=
-  | EvalVal v ρ m :
-    eval_expr (Num v) ρ m (NumV v)
-  | EvalVar x v ρ m :
-    ρ !! x = Some v →
-    eval_expr (Var x) ρ m v
-  | EvalBinOp op e1 e2 v1 v2 v ρ m :
-    eval_expr e1 ρ m v1 →
-    eval_expr e2 ρ m v2 →
-    bin_op_eval op v1 v2 = Some v →
-    eval_expr (BinOp op e1 e2) ρ m v
-  | EvalLoad e v l ρ m :
-    eval_expr e ρ m (LocV l) →
-    m !! l = Some v →
-    eval_expr (UnOp DerefOp e) ρ m v
-  .
-
-Fixpoint exec_eval_expr (e : expr) (ρ : gmap string val) (m : gmap loc val) : option val :=
-  match e with
-  | Num v => Some (NumV v)
-  | Var x => ρ !! x
-  | BinOp op e1 e2 =>
-    v1 ← exec_eval_expr e1 ρ m ;
-    v2 ← exec_eval_expr e2 ρ m ;
-    bin_op_eval op v1 v2
-  | UnOp op e1 =>
-    v1 ← exec_eval_expr e1 ρ m ;
-    match op, v1 with
-    | DerefOp, LocV l =>
-      m !! l
-    | _, _ => None
-    end
-  end.
 
 Definition eval_expr' e s v : Prop := (eval_expr e s.(ρ) s.(m) v).
 Definition eval_exprs' es s vs : Prop :=
