src/lifting.v
@@ -1,9 +1,8 @@
 (* wp for implang *)
 From iris.base_logic Require Import gen_heap.
-From iris.base_logic.lib Require Export fancy_updates.
 From iris_simp_lang Require Import stack_ra implang imp_notation.
 
-Section wp_expr.
+Section wp.
 
 Context `{!gen_heapGS loc val Σ} `{!envGS val Σ} `{!invGS_gen HasNoLc Σ}.
 
@@ -11,26 +10,23 @@ Implicit Types (ρ : @env_state val) (σ : gmap loc val).
 
 Definition state_interp σ ρ := (gen_heap_interp σ ∗ env_auth ρ)%I.
 
-Definition env_match ρ r := λ n, ρ !! n = Some r.
-
-Definition wp_expr_pre (wp : func_env -d> coPset -d> stmt -d> iPropO Σ -d> iPropO Σ) :
+Definition wp_pre (wp : func_env -d> coPset -d> stmt -d> iPropO Σ -d> iPropO Σ) :
     func_env -d> coPset -d> stmt -d> iPropO Σ -d> iPropO Σ := λ F E s Q,
- (
-  ∀ σ ρ n, state_interp σ ρ ={E,∅}=∗ ∀ r, ⌜env_match ρ r n⌝ -∗ ∃ s' r' σ' stk stk',
+ (∀ σ ρ n, state_interp σ ρ ={E,∅}=∗ ∀ r, ⌜env_match ρ r n⌝ -∗ ∃ s' r' σ' stk stk',
         ⌜step F s (Build_state r σ stk) s' (Build_state r' σ' stk')⌝ ∗
         ▷ |={∅,E}=> ∃ ρ', state_interp σ' ρ' ∗ ⌜env_match ρ' r' n⌝ ∗ wp F E s' Q)%I.
 
-Local Instance wp_expr_contractive : Contractive (wp_expr_pre).
+Local Instance wp_contractive : Contractive (wp_pre).
 Proof.
-  rewrite /wp_expr_pre /= => n wp wp' Hwp F E s Q.
+  rewrite /wp_pre /= => n wp wp' Hwp F E s Q.
   do 28 (f_contractive || f_equiv). apply Hwp.
 Qed.
 
-Local Definition wp_expr_def := fixpoint wp_expr_pre.
-Local Definition wp_expr_aux : seal (@wp_expr_def). Proof. by eexists. Qed.
-Definition wp_expr := wp_expr_aux.(unseal).
-Local Lemma wp_expr_unseal   : wp_expr = @wp_expr_def.
-Proof. rewrite -wp_expr_aux.(seal_eq) //. Qed.
+Local Definition wp_def := fixpoint wp_pre.
+Local Definition wp_aux : seal (@wp_def). Proof. by eexists. Qed.
+Definition wp_expr := wp_aux.(unseal).
+Local Lemma wp_unseal   : wp_expr = @wp_def.
+Proof. rewrite -wp_aux.(seal_eq) //. Qed.
 
   
-End wp_expr.
+End wp.
