src/implang_expr.v
@@ -1,0 +1,107 @@
+From stdpp Require Export binders strings.
+From stdpp Require Import gmap.
+From iris.algebra Require Export ofe.
+From iris.prelude Require Import options.
+Open Scope Z.
+From RecordUpdate Require Import RecordSet.
+Import RecordSetNotations.
+
+
+Inductive bin_op :=
+  | PlusOp
+  | EqOp.
+
+Inductive un_op :=
+  | DerefOp.
+
+Inductive expr :=
+  (* Values *)
+  | Num (n : Z)
+  (* local variable *)
+  | Var (x : string)
+  (* Pure operations *)
+  | BinOp (op : bin_op) (e1 e2 : expr)
+  | UnOp (op : un_op) (e : expr)
+.
+
+Bind Scope expr_scope with expr.
+
+(** Equality and other typeclass stuff *)
+
+(*|
+We will now do a bunch of boring work to prove that expressions have decidable
+equality and are countable for technical reasons.
+|*)
+
+Global Instance bin_op_eq_dec : EqDecision bin_op.
+Proof. solve_decision. Defined.
+Global Instance un_op_eq_dec : EqDecision un_op.
+Proof. solve_decision. Defined.
+Lemma expr_eq_dec (e1 e2: expr) : Decision (e1 = e2).
+Proof. solve_decision. Defined.
+Global Instance expr_eq_dec' : EqDecision expr := expr_eq_dec.
+
+Definition Bool (b:bool) : expr := Num (if b then 1 else 0).
+
+(* semantics *)
+Definition loc := Z.
+
+Inductive val :=
+  | NumV (n : Z)
+  | LocV (l : loc).
+
+Lemma val_eq_dec (v1 v2 : val) : Decision (v1 = v2).
+Proof. solve_decision. Defined.
+Global Instance val_eq_dec' : EqDecision val := val_eq_dec.
+
+Definition BoolV (b:bool) : val := NumV (if b then 1 else 0).
+
+Definition bin_op_eval (op: bin_op) (v1 v2: val) : option val :=
+  match op with
+  | PlusOp => match v1, v2 with
+              | NumV n1, NumV n2 =>
+                Some (NumV (n1 + n2))
+              | LocV n1, NumV n2 | NumV n1, LocV n2 =>
+                Some (LocV (n1 + n2))
+              | _, _ => None
+              end
+  | EqOp => Some (BoolV $ bool_decide (v1 = v2))
+  end.
+
+(** the language interface needs these things to be inhabited, I believe *)
+Global Instance val_inhabited : Inhabited val := populate (NumV 0).
+Global Instance expr_inhabited : Inhabited expr := populate (Num 0).
+
+Inductive eval_expr : expr → gmap string val → gmap loc val → val → Prop :=
+  | EvalVal v ρ m :
+    eval_expr (Num v) ρ m (NumV v)
+  | EvalVar x v ρ m :
+    ρ !! x = Some v →
+    eval_expr (Var x) ρ m v
+  | EvalBinOp op e1 e2 v1 v2 v ρ m :
+    eval_expr e1 ρ m v1 →
+    eval_expr e2 ρ m v2 →
+    bin_op_eval op v1 v2 = Some v →
+    eval_expr (BinOp op e1 e2) ρ m v
+  | EvalLoad e v l ρ m :
+    eval_expr e ρ m (LocV l) →
+    m !! l = Some v →
+    eval_expr (UnOp DerefOp e) ρ m v
+  .
+
+Fixpoint exec_eval_expr (e : expr) (ρ : gmap string val) (m : gmap loc val) : option val :=
+  match e with
+  | Num v => Some (NumV v)
+  | Var x => ρ !! x
+  | BinOp op e1 e2 =>
+    v1 ← exec_eval_expr e1 ρ m ;
+    v2 ← exec_eval_expr e2 ρ m ;
+    bin_op_eval op v1 v2
+  | UnOp op e1 =>
+    v1 ← exec_eval_expr e1 ρ m ;
+    match op, v1 with
+    | DerefOp, LocV l =>
+      m !! l
+    | _, _ => None
+    end
+  end.
