src/lifting_expr.v
@@ -1,0 +1,23 @@
+(* wp for implang *)
+From iris.base_logic Require Import gen_heap.
+From iris.base_logic.lib Require Export fancy_updates.
+From iris_simp_lang Require Import stack_ra implang_expr.
+
+Section wp_expr.
+
+Context `{!gen_heapGS loc val Σ} `{!envGS val Σ} `{!invGS_gen HasNoLc Σ}.
+
+Implicit Types (ρ : @env_state val) (σ : gmap loc val).
+
+Definition state_interp σ ρ : assert := (⎡gen_heap_interp σ⎤ ∗ ⎡env_auth ρ⎤)%I.
+
+Definition env_match ρ r := assert_of (λ n, ⌜ρ !! n = Some r⌝)%I.
+
+Definition wp_expr E e Q : assert :=
+  (∀ σ ρ, state_interp σ ρ ={E}=∗
+     ∃ v, (∀ r, env_match ρ r -∗ ⌜eval_expr e r σ v⌝) ∗
+          state_interp σ ρ ∗ Q v)%I.
+
+
+
+End wp_expr.
